ttcan: schedule: fix flaky proofs

example/ttcan/Network.TTCan.Types.Schedule.fst
@@ -5,6 +5,15 @@ module List       = FStar.List.Tot
 
 open FStar.Mul
 
+#push-options "--fuel 1 --ifuel 1"
+
+(*
+  Events are parameterised by abstract "cycle parameters". In the concrete
+  system, the cycle parameters contain the currently-active cycle (the cycle
+  index) and the current ref-trigger-offset, which denotes the time offset for
+  reference messages.
+  Cycle parameters are generally denoted by `c` with type parameter `'c`.
+*)
 
 noeq
 type event_info 'c = {
@@ -29,29 +38,29 @@ type events 'c = {
   exec_period   : pos;
 }
 
-let event_index (evs: events 'c) = n: nat { n <  evs.count }
-let event_count (evs: events 'c) = n: nat { n <= evs.count }
+let event_index_t (evs: events 'c) = n: nat { n <  evs.count }
+let event_count_t (evs: events 'c) = n: nat { n <= evs.count }
 
 (***** Requirements on trigger array ****)
 
 (* Time-marks are sorted *)
-let time_mark_sorted (evs: events 'c) (i j: event_index evs): prop =
+let time_mark_sorted (evs: events 'c) (i j: event_index_t evs): prop =
   (evs.read i).time_mark_max <= (evs.read j).time_mark_min
 
 let time_mark_sorted_all (evs: events 'c): prop =
-  forall (i j: event_index evs).
+  forall (i j: event_index_t evs).
     i <= j ==>
     time_mark_sorted evs i j
 
 (* Adequate time gap between events enabled on same cycle *)
-let adequate_spacing (evs: events 'c) (c: 'c) (i j: event_index evs): prop =
+let adequate_spacing (evs: events 'c) (c: 'c) (i j: event_index_t evs): prop =
   i <= j             ==>
   (evs.read i).enabled c ==>
   (evs.read j).enabled c ==>
   (evs.read j).time_mark_min - (evs.read i).time_mark_max >= (j - i) * evs.exec_period
 
 let adequate_spacing_all (evs: events 'c): prop =
-  forall (c: 'c). forall (i j: event_index evs).
+  forall (c: 'c). forall (i j: event_index_t evs).
     adequate_spacing evs c i j
 
 (* Adequate time gap from start of array to trigger:
@@ -59,11 +68,11 @@ let adequate_spacing_all (evs: events 'c): prop =
   must account for at least (i + 1) steps
   > time_mark(i) : [ (i + 1) * pi, ...)
  *)
-let time_mark_reachable (evs: events 'c) (i: event_index evs): prop =
+let time_mark_reachable (evs: events 'c) (i: event_index_t evs): prop =
     i * evs.exec_period + evs.exec_period <= (evs.read i).time_mark_min
 
 let time_mark_reachable_all (evs: events 'c): prop =
-  forall (i: event_index evs).
+  forall (i: event_index_t evs).
     time_mark_reachable evs i
 
 let events_valid_req (evs: events 'c): prop =
@@ -93,31 +102,31 @@ let time_mark_started (evs: events 'c) (now time_mark: nat): bool =
   > impending_period : [time_mark - pi, time_mark)
   *)
 let time_mark_impending (evs: events 'c) (now time_mark: nat): bool =
-  now <  time_mark + evs.exec_period &&
-  now >= time_mark // - evs.exec_period
+  time_mark_started evs now time_mark &&
+  now <  time_mark + evs.exec_period
 
-let event_enabled_started (evs: events 'c) (c: 'c) (now: nat) (index: event_index evs): bool =
+let event_enabled_started (evs: events 'c) (c: 'c) (now: nat) (index: event_index_t evs): bool =
   let ev = evs.read index in
   ev.enabled c && time_mark_started evs now (ev.time_mark c)
 
 (* Check that there are no enabled triggers inside the given range *)
 let none_enabled (evs: events 'c) (c: 'c) (now: nat) (begin_ end_: int): prop =
-  forall (i: event_index evs { begin_ <= i /\ i < end_ }).
+  forall (i: event_index_t evs { begin_ <= i /\ i < end_ }).
     not ((evs.read i).enabled c)
 
 (* Check that there are no started and enabled triggers inside the given range *)
 let none_started (evs: events 'c) (c: 'c) (now: nat) (begin_ end_: int): prop =
-  forall (i: event_index evs { begin_ <= i /\ i < end_ }).
+  forall (i: event_index_t evs { begin_ <= i /\ i < end_ }).
     let ev = evs.read i in
     ev.enabled c ==> not (time_mark_started evs now (ev.time_mark c))
 
 (* Check that all enabled triggers in the range have started *)
 let all_started (evs: events 'c) (c: 'c) (now: nat) (begin_ end_: int): prop =
-  forall (i: event_index evs { begin_ <= i /\ i < end_ }).
+  forall (i: event_index_t evs { begin_ <= i /\ i < end_ }).
     let ev = evs.read i in
     ev.enabled c ==> time_mark_started evs now (ev.time_mark c)
 
-let lemma_all_started_before (evs: events_valid 'c) (c: 'c) (now: nat) (index: event_index evs)
+let lemma_all_started_before (evs: events_valid 'c) (c: 'c) (now: nat) (index: event_index_t evs)
   : Lemma
     (requires (
       time_mark_started evs now ((evs.read index).time_mark c)
@@ -127,12 +136,12 @@ let lemma_all_started_before (evs: events_valid 'c) (c: 'c) (now: nat) (index: e
     ))
     =
   assert (time_mark_sorted_all evs);
-  assert (forall (i: event_index evs { i <= index }). time_mark_sorted evs i index);
-  assert (forall (i: event_index evs { i <= index }). time_mark_started evs now ((evs.read i).time_mark c));
+  assert (forall (i: event_index_t evs { i <= index }). time_mark_sorted evs i index);
+  assert (forall (i: event_index_t evs { i <= index }). time_mark_started evs now ((evs.read i).time_mark c));
   assert (all_started evs c now 0 (index + 1));
   ()
 
-let lemma_none_started_after (evs: events_valid 'c) (c: 'c) (now: nat) (index: event_index evs)
+let lemma_none_started_after (evs: events_valid 'c) (c: 'c) (now: nat) (index: event_index_t evs)
   : Lemma
     (requires (
       not (time_mark_started evs now ((evs.read index).time_mark c))
@@ -142,23 +151,23 @@ let lemma_none_started_after (evs: events_valid 'c) (c: 'c) (now: nat) (index: e
     ))
     =
   assert (time_mark_sorted_all evs);
-  assert (forall (i: event_index evs { index <= i }). time_mark_sorted evs index i);
-  assert (forall (i: event_index evs { index <= i }). not (time_mark_started evs now ((evs.read i).time_mark c)));
+  assert (forall (i: event_index_t evs { index <= i }). time_mark_sorted evs index i);
+  assert (forall (i: event_index_t evs { index <= i }). not (time_mark_started evs now ((evs.read i).time_mark c)));
   assert (none_started evs c now index evs.count);
   ()
 
-let range_begin_of_option (#evs: events_valid 'c) (nxt: option (event_index evs)): event_count evs =
+let range_begin_of_option (#evs: events_valid 'c) (nxt: option (event_index_t evs)): event_count_t evs =
   match nxt with
   | Some nxt -> nxt + 1
   | None     -> 0
 
-let range_end_of_option (#evs: events_valid 'c) (cur: option (event_index evs)): event_count evs =
+let range_end_of_option (#evs: events_valid 'c) (cur: option (event_index_t evs)): event_count_t evs =
   match cur with
   | Some cur -> cur
   | None     -> evs.count
 
 
-let maximum_started_spec (evs: events_valid 'c) (c: 'c) (now: nat) (cur: option (event_index evs))
+let maximum_started_spec (evs: events_valid 'c) (c: 'c) (now: nat) (cur: option (event_index_t evs))
   : prop =
   all_started  evs c now 0 (range_begin_of_option cur)           /\
   none_started evs c now   (range_begin_of_option cur) evs.count /\
@@ -166,7 +175,7 @@ let maximum_started_spec (evs: events_valid 'c) (c: 'c) (now: nat) (cur: option 
   | Some cur -> (evs.read cur).enabled c
   | None     -> true)
 
-let minimum_not_started_spec (evs: events_valid 'c) (c: 'c) (now: nat)  (cur: option (event_index evs))
+let minimum_not_started_spec (evs: events_valid 'c) (c: 'c) (now: nat)  (cur: option (event_index_t evs))
   : prop =
   all_started  evs c now 0 (range_end_of_option cur)           /\
   none_started evs c now   (range_end_of_option cur) evs.count /\
@@ -174,22 +183,16 @@ let minimum_not_started_spec (evs: events_valid 'c) (c: 'c) (now: nat)  (cur: op
   | Some cur -> (evs.read cur).enabled c
   | None     -> true)
 
-(* Compute the currently-active index for given time (specification only).
-  We want to find the last index that has actually occurred. To do this, we
-  find the next index, and check if that's in the future.
-
-  This function isn't immediately correct on its own. We really
-  need to prove something about it, like that it computes:
-  > maximum i. enabled i /\ (for n in next i. enabled n /\ time_mark n > time)
+(* Compute the currently-active index for given time.
+  This finds the maximum (latest) index that has already started.
 *)
-let rec maximum_started (evs: events_valid 'c) (c: 'c) (now: nat) (index: event_index evs { none_started evs c now (index + 1) evs.count })
+let rec maximum_started (evs: events_valid 'c) (c: 'c) (now: nat) (index: event_index_t evs { none_started evs c now (index + 1) evs.count })
   : Tot
-    (cur: option (event_index evs) {
+    (cur: option (event_index_t evs) {
       maximum_started_spec evs c now cur
     })
     (decreases index) =
-  let ev = evs.read index in
-  if ev.enabled c && time_mark_started evs now (ev.time_mark c)
+  if event_enabled_started evs c now index
   then begin
     lemma_all_started_before evs c now index;
     Some index
@@ -200,11 +203,13 @@ let rec maximum_started (evs: events_valid 'c) (c: 'c) (now: nat) (index: event_
   end
   else None
 
-(* Compute the next-active index for given time (specification only).
+(* Compute the next-active index for given time.
+  This finds the minimum (earliest) index that has is enabled, but not yet
+  started.
 *)
-let rec minimum_not_started (evs: events_valid 'c) (c: 'c) (now: nat) (index: event_index evs { all_started evs c now 0 index })
+let rec minimum_not_started (evs: events_valid 'c) (c: 'c) (now: nat) (index: event_index_t evs { all_started evs c now 0 index })
   : Tot
-    (cur: option (event_index evs) {
+    (cur: option (event_index_t evs) {
       minimum_not_started_spec evs c now cur
     })
     (decreases (evs.count - index)) =
@@ -220,12 +225,14 @@ let rec minimum_not_started (evs: events_valid 'c) (c: 'c) (now: nat) (index: ev
   end
   else None
 
+(* Compute the currently-active event. *)
 let current (evs: events_valid 'c) (c: 'c) (now: nat)
-  : option (event_index evs) =
+  : option (event_index_t evs) =
   maximum_started evs c now (evs.count - 1)
 
+(* Compute the next-active event. *)
 let next (evs: events_valid 'c) (c: 'c) (now: nat)
-  : option (event_index evs) =
+  : option (event_index_t evs) =
   minimum_not_started evs c now 0
 
 let lemma_none_enabled_between
@@ -239,16 +246,17 @@ let lemma_none_enabled_between
     =
   ()
 
-let prefetch_invariant_can_reach_next (evs: events_valid 'c) (c: 'c) (now: nat) (index nxt: event_index evs): bool =
-  let ev = evs.read nxt in
-  let tm = ev.time_mark c in
+let prefetch_invariant_can_reach_next (evs: events_valid 'c) (c: 'c) (now: nat) (index nxt: event_index_t evs): bool =
+  // let ev = evs.read nxt in
+  // let tm = ev.time_mark c in
+
   // need to arrive at time-mark a touch early
   // let tm_early = tm - 1 in
   // steps required to get from current index to next
   // let steps = nxt - index in
-  (nxt - index) * evs.exec_period < tm - now
+  (nxt - index) * evs.exec_period < (evs.read nxt).time_mark c - now
 
-let prefetch_invariant (evs: events_valid 'c) (c: 'c) (now: nat) (index: event_index evs): bool =
+let prefetch_invariant (evs: events_valid 'c) (c: 'c) (now: nat) (index: event_index_t evs): bool =
   (match current evs c now with
     | Some cur -> cur <= index
     | None     -> true) &&
@@ -276,7 +284,7 @@ let lemma_current_reset (evs: events_valid 'c) (c: 'c) (now: nat)
     ()
 
 let lemma_prefetch_invariant_can_reach_next_reset
-  (evs: events_valid 'c) (c: 'c) (now: nat) (next: event_index evs)
+  (evs: events_valid 'c) (c: 'c) (now: nat) (next: event_index_t evs)
   : Lemma
     (requires (
        now < evs.exec_period
@@ -286,6 +294,9 @@ let lemma_prefetch_invariant_can_reach_next_reset
     )) =
   ()
 
+(* Prefetch invariant: reset
+  When the time and index are reset, the invariant is established.
+*)
 let lemma_prefetch_invariant_reset
   (evs: events_valid 'c) (c: 'c) (now: nat)
   : Lemma
@@ -305,14 +316,14 @@ let lemma_prefetch_invariant_reset
 
 (*
   When computing the next not-started event, if:
-  (NXT) we find a result (next ... == Some `nxt`);
+  (NXT) we find a result (next ... == Some nxt);
   (EN) and we know that there is an index `index` that is enabled and not-started;
   (BND) and the index `index` is less than or equal to `nxt`;
 
   then, the next index `nxt` must actually refer to `index`
 *)
 let lemma_next_find
-  (evs: events_valid 'c) (c: 'c) (now: nat) (index nxt: event_index evs)
+  (evs: events_valid 'c) (c: 'c) (now: nat) (index nxt: event_index_t evs)
   : Lemma
     (requires (
       let ev = evs.read index in
@@ -333,14 +344,14 @@ let lemma_next_find
 
 (*
   When computing the next not-started event, if:
-  (TIME) time progresses from now to now' at <=exec_period per tick
+  (TIME) time progresses from now to now' at <=exec_period per tick;
   (NXT) we previously found the next event (next ... now == Some `nxt`);
   (STARTED) and the event is still not started at the updated time now'
 
   then, the next index remains the same at the updated time now'
 *)
 let lemma_next_time_increase
-  (evs: events_valid 'c) (c: 'c) (now now': nat) (nxt: event_index evs)
+  (evs: events_valid 'c) (c: 'c) (now now': nat) (nxt: event_index_t evs)
   : Lemma
     (requires (
       // (TIME)
@@ -380,8 +391,13 @@ let lemma_current_time_increase_next_same
     =
   ()
 
+(* Prefetch invariant maintained: stay
+  When the current index points to an active / enabled event which has not yet
+  started, the prefetch invariant is maintained and the current index remains
+  the same.
+  *)
 let lemma_prefetch_invariant_stay
-  (evs: events_valid 'c) (c: 'c) (now now': nat) (index: event_index evs)
+  (evs: events_valid 'c) (c: 'c) (now now': nat) (index: event_index_t evs)
   : Lemma
     (requires (
       let ev = evs.read index in
@@ -397,8 +413,35 @@ let lemma_prefetch_invariant_stay
     ))
   = ()
 
-let lemma_prefetch_invariant_next_time_increase
-  (evs: events_valid 'c) (c: 'c) (now now': nat) (index: event_index evs)
+let lemma_prefetch_invariant_can_reach_next_skip_same
+  (evs: events_valid 'c) (c: 'c) (now now': nat)
+  (index nxt: event_index_t evs)
+  : Lemma
+    (requires (
+      prefetch_invariant_can_reach_next evs c now index nxt /\
+      next evs c now == Some nxt /\
+      time_period_advances evs now now' /\
+      index < nxt
+    ))
+    (ensures (
+      next evs c now' == Some nxt
+      // let ev = evs.read nxt in
+      // let tm = ev.time_mark c in
+      // ~ (time_mark_started evs now' tm)
+    ))
+  =
+    let ev = evs.read nxt in
+    let tm = ev.time_mark c in
+    assert (~ (time_mark_started evs now  tm));
+    assert (~ (time_mark_started evs now' tm));
+    ()
+
+(* Prefetch invariant: skipping disabled preserves next
+  If the current event is disabled and time passes, then the new next is the
+  same as the old next.
+  *)
+let lemma_prefetch_invariant_next_time_increase_same
+  (evs: events_valid 'c) (c: 'c) (now now': nat) (index: event_index_t evs)
   : Lemma
     (requires (
       time_period_advances evs now now' /\
@@ -411,20 +454,13 @@ let lemma_prefetch_invariant_next_time_increase
     =
   match next evs c now with
   | Some nxt ->
-    let ev = evs.read nxt in
-    let tm = ev.time_mark c in
-    assert (prefetch_invariant_can_reach_next evs c now index nxt);
-    assert (index < nxt);
-    assert (~ (time_mark_started evs now  tm));
-    assert (now < tm);
-    assert (~ (time_mark_started evs now' tm));
-    assert (next evs c now' == Some nxt);
+    lemma_prefetch_invariant_can_reach_next_skip_same evs c now now' index nxt;
     ()
   | None ->
     ()
 
 let lemma_prefetch_invariant_skip
-  (evs: events_valid 'c) (c: 'c) (now now': nat) (index: event_index evs)
+  (evs: events_valid 'c) (c: 'c) (now now': nat) (index: event_index_t evs)
   : Lemma
     (requires (
       let ev = evs.read index in
@@ -439,28 +475,21 @@ let lemma_prefetch_invariant_skip
       prefetch_invariant evs c now' (index + 1)
     ))
   =
-  lemma_prefetch_invariant_next_time_increase evs c now now' index;
+  lemma_prefetch_invariant_next_time_increase_same evs c now now' index;
   assert (next evs c now    == next evs c now');
   assert (current evs c now == current evs c now');
-  // (match next evs c now with
-  //   | Some nxt ->
-  //     index <= nxt &&
-  //     prefetch_invariant_can_reach_next evs c now index nxt
-  //   | None     -> true);
   ()
 
 let lemma_enabled_time_lt
   (evs: events_valid 'c) (c: 'c)
-  (index: event_index evs)
-  (i: event_index evs { index < i })
+  (index: event_index_t evs)
+  (i: event_index_t evs { index < i })
   : Lemma
     (requires (
       (evs.read index).enabled c /\
       (evs.read i).enabled c
     ))
     (ensures (
-      // forall (i: event_index evs { index < i}).
-      // (evs.read i).enabled c ==>
       (evs.read index).time_mark c < (evs.read i).time_mark c
     ))
     =
@@ -468,9 +497,26 @@ let lemma_enabled_time_lt
   assert (adequate_spacing evs c index i);
   ()
 
+let lemma_time_mark_both_enabled_gap
+  (evs: events_valid 'c) (c: 'c) (now now': nat)
+  (i i': event_index_t evs)
+  : Lemma
+    (requires (
+      i < i'
+    ))
+    (ensures (
+      (evs.read i).enabled c ==>
+      (evs.read i').enabled c ==>
+      ((evs.read i).time_mark c + evs.exec_period <= (evs.read i').time_mark c)
+    ))
+    =
+  assert (time_mark_sorted evs i i');
+  assert (adequate_spacing evs c i i');
+  ()
+
 let lemma_current_time_increase_start
   (evs: events_valid 'c) (c: 'c) (now now': nat)
-  (index: event_index evs)
+  (index: event_index_t evs)
   : Lemma
     (requires (
       let ev = evs.read index in
@@ -490,18 +536,41 @@ let lemma_current_time_increase_start
     assert (all_started evs c now' 0 cur);
     assert (none_started evs c now' (cur + 1) evs.count);
     assert (index <= cur);
-    assert (forall (i: event_index evs { index < i }). time_mark_sorted evs index i);
-    assert (forall (i: event_index evs { index < i }). adequate_spacing evs c index i);
-    assert (forall (i: event_index evs { index < i }). tm <= (evs.read i).time_mark c);
-    assert (forall (i: event_index evs { index < i }). (evs.read i).enabled c ==> tm < ((evs.read i).time_mark c));
-    assert (forall (i: event_index evs { index < i }). (evs.read i).enabled c ==> ~ (time_mark_started evs now' ((evs.read i).time_mark c)));
+    introduce forall (i: event_index_t evs { index < i }). (evs.read i).enabled c ==> ~ (time_mark_started evs now' ((evs.read i).time_mark c))
+    with begin
+      lemma_time_mark_both_enabled_gap evs c now now' index i;
+      // assert (time_mark_sorted evs index i);
+      // assert (adequate_spacing evs c index i);
+      // assert (tm <= (evs.read i).time_mark c);
+      // assert ((evs.read i).enabled c ==> tm < ((evs.read i).time_mark c));
+      // assume ((evs.read i).enabled c ==> tm + evs.exec_period <= ((evs.read i).time_mark c));
+      // FLAKY
+      // assert (~ (now >= tm));
+      // assert ((now' >= tm));
+      // assert (~ (now >= (evs.read i).time_mark c));
+      // assert ((evs.read i).enabled c ==> (tm < (evs.read i).time_mark c));
+      // assert ((evs.read i).enabled c ==> ~ (now' >= (evs.read i).time_mark c));
+      // assert ((evs.read i).enabled c ==> ~ (time_mark_started evs now' ((evs.read i).time_mark c)));
+      ()
+    end;
+
+    // introduce forall (i: event_index_t evs { index < i }).
+    // assert (forall (i: event_index_t evs { index < i }). time_mark_sorted evs index i);
+    // assert (forall (i: event_index_t evs { index < i }). adequate_spacing evs c index i);
+    // assert (forall (i: event_index_t evs { index < i }). tm <= (evs.read i).time_mark c);
+    // assert (forall (i: event_index_t evs { index < i }). (evs.read i).enabled c ==> tm < ((evs.read i).time_mark c));
+    // // FLAKY
+    // assert (not (now >= tm));
+    // assert (forall (i: event_index_t evs { index < i }). (evs.read i).enabled c ==> (evs.read i).time_mark c > now);
+    // assume (forall (i: event_index_t evs { index < i }). (evs.read i).enabled c ==> ~ (time_mark_started evs now' ((evs.read i).time_mark c)));
     assert (cur == index)
   | None ->
     false_elim ()
 
+
 let lemma_prefetch_invariant_can_reach_next_time_increase
   (evs: events_valid 'c) (c: 'c) (now now': nat)
-  (index nxt': event_index evs)
+  (index nxt': event_index_t evs)
   : Lemma
     (requires (
       let ev = evs.read index in
@@ -518,14 +587,26 @@ let lemma_prefetch_invariant_can_reach_next_time_increase
     =
   let ei = evs.read index in
   let en = evs.read nxt' in
+  let ti = ei.time_mark c in
+  let tn = en.time_mark c in
   assert (adequate_spacing evs c index nxt');
-  assert (ei.time_mark c < en.time_mark c);
-  assert ((en.time_mark c - ei.time_mark c) >= (nxt' - index) * evs.exec_period);
-  assert (prefetch_invariant_can_reach_next evs c now' (index + 1) nxt');
+  assert (index <= nxt' /\ ei.enabled c /\ en.enabled c);
+  assert (en.time_mark_min - ei.time_mark_max >= (nxt' - index) * evs.exec_period);
+  assert (en.time_mark_min <= tn);
+  assert (ti <= ei.time_mark_max);
+  assert (ti < tn);
+  assert (tn - ti >= (nxt' - index) * evs.exec_period);
+  assert (now < ti);
+  assert (ti <= now');
+  // FLAKY
+  assert ((nxt' - index) * evs.exec_period - evs.exec_period < tn - now');
+  // assert ((nxt' - index) * evs.exec_period < tn - now' + evs.exec_period);
+  // assert ((nxt' - (index + 1)) * evs.exec_period < tn - now');
+  // assert (prefetch_invariant_can_reach_next evs c now' (index + 1) nxt');
   ()
 
 let lemma_prefetch_invariant_done
-  (evs: events_valid 'c) (c: 'c) (now now': nat) (index: event_index evs)
+  (evs: events_valid 'c) (c: 'c) (now now': nat) (index: event_index_t evs)
   : Lemma
     (requires (
       let ev = evs.read index in
@@ -556,13 +637,11 @@ let lemma_prefetch_invariant_done
 
 
 let lemma_prefetch_invariant_end
-  (evs: events_valid 'c) (c: 'c) (now now': nat) (index: event_index evs)
+  (evs: events_valid 'c) (c: 'c) (now now': nat) (index: event_index_t evs)
   : Lemma
     (requires (
       time_period_advances evs now now' /\
-
       index == evs.count - 1 /\
-
       prefetch_invariant evs c now  index
     ))
     (ensures (
